module name refactoring + minor tweaks to some Example Phrases

src/extra/Cvm_Impl.hs
@@ -1,0 +1,40 @@
+module Impl_VM where
+
+import qualified Prelude
+import qualified Anno_Term_Defs
+import qualified GenStMonad
+import qualified MonadVM
+import qualified StVM
+
+copland_compile :: Anno_Term_Defs.AnnoTermPar -> StVM.CVM ()
+copland_compile t =
+  case t of {
+   Anno_Term_Defs.Coq_aasp_par a ->
+    GenStMonad.bind (MonadVM.do_prim a) MonadVM.put_ev;
+   Anno_Term_Defs.Coq_aatt_par q t' ->
+    GenStMonad.bind MonadVM.get_ev (\e ->
+      GenStMonad.bind (MonadVM.doRemote t' q e) MonadVM.put_ev);
+   Anno_Term_Defs.Coq_alseq_par t1 t2 ->
+    GenStMonad.bind (copland_compile t1) (\_ -> copland_compile t2);
+   Anno_Term_Defs.Coq_abseq_par sp t1 t2 ->
+    GenStMonad.bind (MonadVM.split_ev sp) (\pr ->
+      case pr of {
+       (,) e1 e2 ->
+        GenStMonad.bind (MonadVM.put_ev e1) (\_ ->
+          GenStMonad.bind (copland_compile t1) (\_ ->
+            GenStMonad.bind MonadVM.get_ev (\e1r ->
+              GenStMonad.bind (MonadVM.put_ev e2) (\_ ->
+                GenStMonad.bind (copland_compile t2) (\_ ->
+                  GenStMonad.bind MonadVM.get_ev (\e2r ->
+                    MonadVM.join_seq e1r e2r))))))});
+   Anno_Term_Defs.Coq_abpar_par loc sp t1 t2 ->
+    GenStMonad.bind (MonadVM.split_ev sp) (\pr ->
+      case pr of {
+       (,) e1 e2 ->
+        GenStMonad.bind (MonadVM.start_par_thread loc t2 e2) (\_ ->
+          GenStMonad.bind (MonadVM.put_ev e1) (\_ ->
+            GenStMonad.bind (copland_compile t1) (\_ ->
+              GenStMonad.bind MonadVM.get_ev (\e1r ->
+                GenStMonad.bind (MonadVM.wait_par_thread loc t2 e2) (\e2r ->
+                  MonadVM.join_par e1r e2r)))))})}
+
