src/extra/GenOptMonad.hs
@@ -1,0 +1,20 @@
+module GenOptMonad where
+
+import qualified Prelude
+
+type Opt a = Prelude.Maybe a
+
+ret :: a1 -> Opt a1
+ret a =
+  Prelude.Just a
+
+bind :: (Opt a1) -> (a1 -> Opt a2) -> Opt a2
+bind m f =
+  case m of {
+   Prelude.Just v -> f v;
+   Prelude.Nothing -> Prelude.Nothing}
+
+failm :: Opt a1
+failm =
+  Prelude.Nothing
+
