src/extra/GenStMonad.hs
@@ -1,0 +1,35 @@
+module GenStMonad where
+
+import qualified Prelude
+import qualified Datatypes
+
+type St s a = s -> (,) (Prelude.Maybe a) s
+
+ret :: a2 -> St a1 a2
+ret a s =
+  (,) (Prelude.Just a) s
+
+bind :: (St a1 a2) -> (a2 -> St a1 a3) -> St a1 a3
+bind m f s =
+  case m s of {
+   (,) a s' ->
+    case a of {
+     Prelude.Just v -> f v s';
+     Prelude.Nothing -> (,) Prelude.Nothing s'}}
+
+modify :: (a1 -> a1) -> St a1 ()
+modify f s =
+  (,) (Prelude.Just ()) (f s)
+
+put :: a1 -> St a1 ()
+put s _ =
+  (,) (Prelude.Just ()) s
+
+get :: St a1 a1
+get s =
+  (,) (Prelude.Just s) s
+
+execSt :: (St a1 a2) -> a1 -> a1
+execSt h s =
+  Datatypes.snd (h s)
+
