src/Appraisal_AltImpls_Eq.v
@@ -1,5 +1,5 @@
 Require Import Event_system Term_system ConcreteEvidence Appraisal_Evidence.
-Require Import Impl_VM Helpers_VmSemantics VmSemantics.
+Require Import Cvm_Impl Helpers_CvmSemantics CvmSemantics.
 Require Import Axioms_Io External_Facts Auto AutoApp Defs.
 
 Require Import Appraisal_Defs Impl_appraisal Impl_appraisal_alt (*MonadAM*).
@@ -17,9 +17,9 @@ Require Import Lia.
 
 Lemma appraisal_alt : forall ec1 ec2 ec2' ls et,
 
-  Some ec1 = Impl_appraisal_alt.build_app_comp_evC et ls ->
+  Some ec1 = Impl_appraisal.build_app_comp_evC et ls ->
   reconstruct_evP (evc ls et) ec2 ->
-  ec2' = Impl_appraisal.build_app_comp_evC ec2 ->
+  ec2' = Impl_appraisal_alt.build_app_comp_evC ec2 ->
   ec1 = ec2'.
 Proof.
   intros.
@@ -31,28 +31,28 @@ Proof.
   -
     do_inv_recon.
     repeat ff.
-    unfold GenOptMonad.bind in *.
-    unfold GenOptMonad.ret in *.
+    unfold OptMonad_Coq.bind in *.
+    unfold OptMonad_Coq.ret in *.
     repeat ff.
     unfold checkNonceF.
     jkjke.
   -
     do_inv_recon.
     repeat ff.
-    unfold GenOptMonad.bind in *.
-    unfold GenOptMonad.ret in *.
+    unfold OptMonad_Coq.bind in *.
+    unfold OptMonad_Coq.ret in *.
     repeat ff.
     
     repeat ff.
 
-    assert (e = (Impl_appraisal.build_app_comp_evC ec2)).
+    assert (e = (Impl_appraisal_alt.build_app_comp_evC ec2)).
     {
       eapply IHec2.
       jkjke.
       invc H0.
       repeat ff.
-      unfold GenOptMonad.bind in *.
-      unfold GenOptMonad.ret in *.
+      unfold OptMonad_Coq.bind in *.
+      unfold OptMonad_Coq.ret in *.
       repeat ff.
       econstructor.
       ff.
@@ -66,11 +66,11 @@ Proof.
     do_recon_inv.
     
     repeat ff.
-    unfold GenOptMonad.bind in *.
-    unfold GenOptMonad.ret in *.
+    unfold OptMonad_Coq.bind in *.
+    unfold OptMonad_Coq.ret in *.
     repeat ff.
 
-    assert (e = (Impl_appraisal.build_app_comp_evC ec2)) by eauto.
+    assert (e = (Impl_appraisal_alt.build_app_comp_evC ec2)) by eauto.
     subst.
     unfold checkSig.
     unfold checkSigF.
@@ -95,8 +95,8 @@ Proof.
   -
     do_inv_recon.
     repeat ff.
-    unfold GenOptMonad.bind in *.
-    unfold GenOptMonad.ret in *.
+    unfold OptMonad_Coq.bind in *.
+    unfold OptMonad_Coq.ret in *.
     repeat ff.
     unfold checkHashF.
     jkjke.
@@ -104,21 +104,21 @@ Proof.
     do_inv_recon.
     do_recon_inv. 
     repeat ff.
-    unfold GenOptMonad.bind in *.
-    unfold GenOptMonad.ret in *.
+    unfold OptMonad_Coq.bind in *.
+    unfold OptMonad_Coq.ret in *.
     repeat ff.
-    assert (e = (Impl_appraisal.build_app_comp_evC ec2_1)) by eauto.
-    assert (e0 = (Impl_appraisal.build_app_comp_evC ec2_2)) by eauto. 
+    assert (e = (Impl_appraisal_alt.build_app_comp_evC ec2_1)) by eauto.
+    assert (e0 = (Impl_appraisal_alt.build_app_comp_evC ec2_2)) by eauto. 
     congruence.
 
   -
     do_inv_recon.
     do_recon_inv.
     repeat ff.
-    unfold GenOptMonad.bind in *.
-    unfold GenOptMonad.ret in *.
+    unfold OptMonad_Coq.bind in *.
+    unfold OptMonad_Coq.ret in *.
     repeat ff.
-    assert (e = (Impl_appraisal.build_app_comp_evC ec2_1)) by eauto.   
-    assert (e0 = (Impl_appraisal.build_app_comp_evC ec2_2)) by eauto.
+    assert (e = (Impl_appraisal_alt.build_app_comp_evC ec2_1)) by eauto.   
+    assert (e0 = (Impl_appraisal_alt.build_app_comp_evC ec2_2)) by eauto.
     congruence.
 Defined.
