src/Example_Phrases_Admits.v
@@ -9,11 +9,25 @@ Admitted.
 Definition cert_id : ASP_ID.
 Admitted.
 
+Definition cache_id : ASP_ID.
+Admitted.
+(*
 Definition store_id : ASP_ID.
 Admitted.
 
 Definition retrieve_id : ASP_ID.
 Admitted.
+*)
+
+
+
+Definition store_args : list Arg.
+Admitted.
+
+Definition retrieve_args : list Arg.
+Admitted.
+
+
 
 Definition sys : TARG_ID.
 Admitted.
