src/IO_Stubs.v
@@ -1,4 +1,4 @@
-Require Import Term_Defs ConcreteEvidence GenStMonad IO_Type.
+Require Import Term_Defs ConcreteEvidence StMonad_Coq IO_Type.
 
 Definition encodeEvRaw(e:RawEv): BS.
 Admitted.
